\section{Perturbation Theory}
\begin{framed}\noindent
  A \red{perturbation} applied to a system

  \begin{equation}
    \label{eqn:pertHamiltonian}
    \hat{H}(t) = \hat{H}_0+\red{\lambda\hat{V}(t)}.
  \end{equation}
  \noindent We  need to find the  evolution of the initial  state to the
  final state
  \begin{equation}
    \ket{\psi(0)} \ira \ket{\psi(t)}.
  \end{equation}

  \noindent  \textbf{We use  eigenstates  $\ket{\phi}_i$  of the  Hermetian
    operator $\hat{H}_0$ that form a basis.}

\end{framed}

\begin{enumerate}
\item The state at an arbitrary time is a weighted superposition
  \begin{equation}
    \label{eqn:pertStates}
    \begin{aligned}
      \ket{\psi(t)}_I & = \sum_j c_j(t)\ket{\phi_j}\qquad\hfill\text{interaction picture - operator evolves}\\
      \ket{\psi(t)}_S               &                =               \sum_j
      c_j(t)\exp\left[\frac{-iE_j\hbar}{t}\right]\ket{\phi_j}\qquad
      \hfill\text{Schrodinger picture - state evolves}
    \end{aligned}
  \end{equation}
\item Solving the  \schrodinger equation in the  iteraction picture (see
  Chapter~\ref{sec:interaction})
  \begin{equation}
    \begin{aligned}
      i\hbar\ipartial{\ket{\psi(t)}_I}{t} & = \bigg(U_0^\dagger\lambda\hat{V}(t)U_0\bigg)\ket{\psi(t)}_I \Rightarrow\\
      i\hbar\ipartial{}{t}\bigg[\sum_j c_j(t)\ket{\phi_j}\bigg] & = \bigg(U_0^\dagger\lambda\hat{V}(t)U_0\bigg)\bigg[\sum_k c_k(t)\ket{\phi_k}\bigg]\\
    \end{aligned}.
  \end{equation}
\item Taking out the time dependent terms, and `sandwiching'
  \begin{equation}
    \begin{aligned}
      \sum_j \ipartial{c_j(t)}{t}\textcolor{red}{\bra{\phi_m}}\ket{\phi_j} & = \frac{\lambda}{i\hbar} \sum_k \bigg[ \textcolor{red}{\bra{\phi_m}}U_0^\dagger\bigg]\hat{V}(t)c_k(t)\bigg[U_0\ket{\phi_k}\bigg]\Rightarrow\\
      \sum_j \ipartial{c_j(t)}{t}\ \delta_{\red{m}j} & = \frac{\lambda}{i\hbar} \sum_k \bigg[ \textcolor{red}{\bra{\phi_m}}e^{+i\red{E_m}t/\hbar}]\hat{V}(t)c_k(t)\bigg[e^{-iE_kt/\hbar}\ket{\phi_k}\bigg] \Rightarrow\\
    \end{aligned}
  \end{equation}
  \noindent where we used
  \begin{equation}
    U(t)\ket{\psi(t)} = \exp[-i\hat{H}t/\hbar]\ket{\psi} = \sum_n\frac{1}{n!}\bigg[\frac{-i\hat{H}t}{\hbar}\bigg]^n\ket{\psi} = \sum_n\frac{1}{n!}\bigg[\frac{-iEt}{\hbar}\bigg]^n\ket{\psi} = \exp[-iEt/\hbar]\ket{\psi}.
  \end{equation}
\item This evaluates to
  \begin{equation}\label{eqn:use}
    \begin{aligned}
      \ipartial{c_{\red{m}}(t)}{t} & = \frac{\lambda}{i\hbar} \sum_k c_k(t)e^{i(\red{E_m}-E_k)t/\hbar} \red{\bra{\phi_m}}\hat{V}(t)\ket{\phi_k}\Rightarrow\\
      \ipartial{c_{\red{m}}(t)}{t}    &   =    \frac{\lambda}{i\hbar}   \sum_k
      c_k(t)e^{i(\red{E_m}-E_k)t/\hbar}
      \left\langle\hat{V}(t)\right\rangle_{\red{m}k}.
    \end{aligned}
  \end{equation}
\item A  useful thing to  do now, is  to expand the  `weighting factors'
  $ c_m(t) $ as a power series of the small parameter $ \lambda $:

  \begin{framed}\noindent
    \begin{equation}\label{expansion}
      c_{m}(t) = c_{m}^{(0)}(t)+\lambda c_{m}^{(1)}(t)+\lambda^2c_m^{(2)}(t)+\cdots
    \end{equation}
  \end{framed}
  \vspace{-1em}

  \textbf{\noindent   Now    lets   sub    in   this    expansion   into
    Eq.~\ref{eqn:use} and compare terms with $ \lambda $ powers on the LHS and
    RHS}:
  \begin{enumerate}
  \item
    \begin{equation}
      \mathbf{\lambda^{0}} \ira \frac{dc^{(0)}_m(t)}{dt} = 0.
    \end{equation}
    \noindent The  initial state of  the system before  any perturbation
    ($       \lambda      =       0       $)       is      an       eigenstate
    $   \iket{\Psi(0)}~=~\iket{\phi_i}  $.    Since  this   initial  weight
    $ c_j^{(0)} $ doesn't change:

    \begin{framed}\noindent
      \begin{equation}\label{lam0}
        \red{\mathbf{c^{(0)}_m}(t)    =    \text{    constant    }    =
          \braket{\phi_m|\Psi(0)} = \delta_{m,i}.}
      \end{equation}
    \end{framed}

  \item $ \mathbf{\lambda^{1}} $
    \begin{equation}\label{lam1}
      \begin{aligned}
        \frac{dc^{(1)}_m(t)}{dt} & = \frac{1}{i\hbar}\sum_{k}c_{k}^{(0)}(t)e^{i\omega_{mk}t} \left\langle\hat{V}(t)\right\rangle_{mk}\\
        & = \frac{1}{i\hbar}\sum_{k}\delta_{k,i}e^{i\omega_{mk}t} \left\langle\hat{V}(t)\right\rangle_{mk}\\
        & = \frac{1}{i\hbar}e^{i\omega_{mi}t} \left\langle\hat{V}(t)\right\rangle_{mi}\\
      \end{aligned}
    \end{equation}

    \noindent giving  weights of  the for  the initial  state component,
    $ c_i^{(1)}(t) $ and the others that arise, $ c_m^{(1)}(t) $:

    \begin{framed}\noindent

      \begin{equation}
        \begin{aligned}
          c_{i}^{(1)}(\tau) & = \frac{1}{i\hbar}\int_{0}^{\tau}dt\hat{V}_{ii}(t)\\
          c_{m}^{(1)}(\tau)                       &                       =
          \frac{1}{i\hbar}\int_{0}^{\tau}dt\hat{V}_{mi}(t)\exp\left[i\omega_{mi}t\right]
        \end{aligned}
      \end{equation}

    \end{framed}
  \end{enumerate}
\end{enumerate}
\noindent

\noindent

\begin{enumerate}

\item $ \mathbf{\lambda^{2}} $
  \begin{equation}\label{lam2}
    \begin{aligned}
      \frac{dc^{(2)}_m(t)}{dt} & = \frac{1}{i\hbar}\sum_{k}c_{k}^{(1)}(t)e^{i\omega_{mk}t} \left\langle\hat{V}(t)\right\rangle_{mk}\\
      &                                                                =
      \frac{1}{i\hbar}\sum_{k}\bigg[\frac{1}{i\hbar}\int_{0}^{t}dt\hat{V}_{mi}(t)\exp\left[i\omega_{mi}t\right]\bigg]e^{i\omega_{mk}t}
      \left\langle\hat{V}(t)\right\rangle_{mk}
    \end{aligned}
  \end{equation}

\end{enumerate}

\subsection{Fermi's golden rule}
\begin{framed}\noindent
  So up  to this point,  we have determined  that we have  the evolution
  following a perturbation in the interactin picture

  \begin{equation}
    \begin{aligned}
      \ket{i} & \ira \iket{\Psi(t)} = \sum_m c_m(t)\ket{m} \equiv \iket{i} + \sum_m c_{m}^{(1)}(t)\iket{m}\\
      & c_{m}(t) = c_{m}^{(0)}(t)+\lambda c_{m}^{(1)}(t)+\lambda^2c_m^{(2)}(t)+\cdots\\
      & c_{m}^{(0)}(t) = \text{ const } = \delta_{m,i}\\
      & c_{i}^{(1)}(\tau) = \frac{1}{i\hbar}\int_{0}^{\tau}dt\hat{V}_{ii}(t)\\
      &                         c_{m}^{(1)}(\tau)                         =
      \frac{1}{i\hbar}\int_{0}^{\tau}dt\hat{V}_{mi}(t)\exp\left[i\omega_{mi}t\right]
    \end{aligned}
  \end{equation}

\end{framed}

\noindent The probability that upon  measurement, we collapse into state
\iket{j}:

\begin{equation}
  \begin{aligned}
    \text{Prob(collapsing      into      $      \iket{j}      $)}      =
    \iabsSquared{\bra{j}\ket{\Psi(t)}}                                    =
    \iabsSquared{\bra{j}\left(\red{\ket{i}}     +    \blue{\lambda\sum_m
          c_{m}^{(1)}(t)\iket{m}}\right)}.
  \end{aligned}
\end{equation}

\noindent  The  \red{first  term}  goes to  zero,  as  states  \iket{i},
\iket{j}   are   othogonal,  and   in   the   \blue{second  term}   only
\iket{m}=\iket{j} will be selected:

\begin{framed}\noindent
  \begin{equation}
    \begin{aligned}
      \text{Prob collapsing into $ \iket{j} $} & = \iabsSquared{\lambda c_j^{(1)}(t)}\\
      & c_j^{(1)}(t) = \frac{1}{i\hbar}\int_{0}^{\tau}dt\hat{V}_{mi}(t)\exp\left[i\omega_{ji}t\right]\\
      & \hat{V}_{ji}(t) = \bra{j}\hat{V}(t)\iket{i}
    \end{aligned}
  \end{equation}
\end{framed}

\red{\textbf{In the special case, that  the perturbation has a frequency
    corresponding  to   the  energy   separation  of   states  \iket{i},
    \iket{j}}}:
\begin{equation}
  \lambda \hat{V}(t) = {\hat{A}}e^{-i\omega_{ji} t},
\end{equation}

\noindent the rotation in the integral cancels out, leaving:
\begin{equation}
  \begin{aligned}
    \text{Prob    collapsing     into    $     \iket{j}    $}     &    =
    \iabsSquared{\frac{1}{i\hbar}\bra{j}\hat{A}\ket{i}\tau}       &       \propto
    \iabsSquared{\bra{j}\hat{A}\ket{i}}.
  \end{aligned}
\end{equation}

\begin{framed}\noindent
  Driving something in  resonane between two states, will  mean that the
  probability of transition (transition rate) is proprtional to
  \begin{equation}
    t_{ij} \propto \iabsSquared{\bra{j}\hat{A}\ket{i}}.
  \end{equation}

\end{framed}
