% -*- TeX-master: "../all_the_notes.tex" -*-

\section{Transmission line}

We treat the  transmission line as a chain of  inductors and capacitors
and that  is lossless  (i.e $  R=0 $  and $ G  = 0  $ =  no conductance
between the lines) with

  \begin{equation}
    l \approx \mu_0 \text{ - the inductance per unit length}\qquad c \approx \epsilon_0 \text{ - the capacitance per unit length},
  \end{equation}

  \noindent as shown in Fig.\ref{transtLine}.  Recall that for a device
  of     size     $     \alpha     $,    the     capacitance     will     be
  $ C  \approx \epsilon_0\alpha $.  The  current and the voltage  in the line
  will have components going in opposite directions

  \begin{equation}
    \label{tlineCurrentVoltage}
    \mathbf{V_{\pm} = V_0e^{\pm ikx-i\omega t};\qquad I_{\pm} = I_0e^{\pm ikx-i\omega t}},
  \end{equation}

  \noindent and be related to each other via the complex impedance

 \begin{equation}
   V_{\pm}= \pm ZI_{\pm}
 \end{equation}

 \begin{figure}
   \caption{ \label{transtLine}}
   \includegraphics[height=3cm]{tline}
 \end{figure}

 \noindent  We  write  the  following equations  from  their  classical
 analogues

 \begin{equation}
   \left\lbrace \begin{aligned}
       V & = -\frac{d\Phi}{dt} = -L\frac{dI}{dt}\\
       I & = -\frac{dQ}{dt} = -C\frac{dV}{dt}
     \end{aligned}\right.\Rightarrow \text{ per unt length} \Rightarrow
   \left\lbrace \begin{aligned}
       \frac{dV}{dx} & = - l\frac{dI}{dt}\\
       \frac{dI}{dx} & - c\frac{dV}{dt},
     \end{aligned}\right.
   \label{tlineDiff}
 \end{equation}

 \begin{itemize}
 \item     We     substitute    Eq.\eqref{tlineCurrentVoltage}     into
   Eq.\eqref{tlineDiff} to get

  \begin{equation}
    \left\lbrace \begin{aligned}
        ikV_0&=i\omega lI_0\\
        -i\omega I_0 & = -ickV_0
      \end{aligned}\right. \Rightarrow\left\lbrace \begin{aligned}
        Z_0&=\frac{V_0}{I_0} = \frac{\omega l }{k}\\
        Z_0&=\frac{V_0}{I_0} = \frac{k}{\omega c}\\
      \end{aligned}\right.  \Rightarrow \red{\mathbf{Z_0 = \sqrt{\frac{l}{c}}}}\approx
    100\Omega
  \end{equation}

\item We differentiate Eq.\eqref{tlineDiff}

  \begin{equation}
    \frac{d^2V}{dx^2} = -l\frac{d^2I}{dt\partial x} = -l\bigg(-c\frac{d^2V}{dt^2}\bigg) \Rightarrow V_{xx} = \frac{1}{1/lc}V_{tt},
  \end{equation}

  \noindent  which  has  the  exact  same form  as  the  wave  equation
  $ y_{xx}=\frac{1}{v^2}y_{tt} $,  from which one can get  the speed of
  wave propagation

  \begin{equation}
    \red{v=\frac{1}{\sqrt{lc}}}
  \end{equation}
\end{itemize}

\begin{figure}
  \caption{\label{tlineres1}}
  \includegraphics[height=4cm]{res1}
\end{figure}

So far we have had a transmission line with no boundary conditions. But
now lets us look at a resonator,  depicted in figure which has two ends
which are cut off and at which

\begin{itemize}
\item \textbf{The current $ I=0 $}:  no charge may flow at these points
  of cut.
\end{itemize}

Mathematically speaking

 \begin{equation}
   \left\lbrace \begin{aligned}
       I(x=0) & = I_{+}(x=0)+I_-(x=0)=0\\
       I(x=L) & = I_{+}(x=L)+I_-(x=L)=0
     \end{aligned}\Rightarrow\begin{aligned}
       \red{I_+}&\red{=-I_-}\\
       I_+&= -I_-e^{-i2kL}
     \end{aligned} \Rightarrow \red{k=\frac{\pi n}{L}}, \right.
 \end{equation}

 \noindent and the total current at  any point in the resonator will be
 a point on a standing wave

 \begin{equation}
   I(x,t) = I_+(x,t) + I_-(x,t) = I_+e^{i\frac{\pi n}{L}x-i\omega t} - I_+e^{-i\frac{\pi n}{L}x-i\omega t} = {{I_0\sin\bigg[\frac{\pi n}{L}x\bigg]e^{-i\omega t}}}.
   \label{tlineCurrent}
 \end{equation}

 \noindent  Evaluating  the   voltage  using  Eq.\eqref{tlineDiff}  and
 Eq.\eqref{tlineCurrent}

 \begin{equation}
   \begin{aligned}
     \frac{dI}{dx} &= - c\frac{dV}{dt}\\
     kI_0\cos(kx)e^{-i\omega t}& =-c\frac{dV}{dt}\\
     \frac{-1}{i\omega}kI_0\cos(kx)e^{-i\omega t}& =-cV\\
     & \Rightarrow\qquad V &=  -i\frac{k}{\omega c}I_0\cos(kx)e^{-i\omega t}\\
     &&=|Z|I_0\cos(kx)e^{-i\omega t}e^{-i\pi/2}\\
     &&=V_0\cos \bigg(\frac{\pi n}{L}x\bigg)\exp\bigg[-i\omega t-i\pi/2\bigg]\\
   \end{aligned}
 \end{equation}

 \noindent or fully the result is (and depicted in Fig.\ref{tlineVI})

 \red{ \begin{equation}
     \begin{aligned}
       V & =V_0\cos \bigg(\frac{\pi n}{L}x\bigg)\exp\bigg[-i\omega t-i\frac{\pi}{2}\bigg]\\
       I & =I_0\sin \bigg(\frac{\pi n}{L}x\bigg)\exp\bigg[-i\omega t\bigg]\\
       V_0&=|Z|I_0
     \end{aligned}
   \end{equation}}

 \begin{figure}
   \includegraphics[height=7cm]{vires}
   \caption{Voltage has  an anti-node at  the two sides,  while current
     has  a   node.   Multiple   modes  can   be  accomodated   by  the
     resonator\label{tlineVI}}
 \end{figure}

 \subsection{The voltages at the gaps of the resonator}
 Now when we consider a boundary, we  shall label + as moving towards a
 boundary,  and -  as moving  away.  By  defining the  transmission and
 reflection as

 \begin{equation}
   t=\frac{|V_{R}^{-}|}{|V_{L}^{+}|};\quad r=\frac{|V_{L}^{-}|}{|V_{L}^{+}|};\quad t=1+r,
 \end{equation}

 \noindent we shall write the propagating waves as follows

 \begin{align}
   V_L^{+} & = V_0e^{ikx-i\omega t}\\
   V_L^{-} & = rV_0e^{\red{-}ikx-i\omega t}\\
   V_R^{+} & = tV_0e^{ikx-i\omega t},
 \end{align}

 \noindent where we assume that no wave is incident from the right hand
 side ($ V_R^{+}=0 $).  Recalling Eq.\eqref{tlineDiff} that relates the
 current  to  the voltage  in  a  line,  let  us evaluate  the  current
 corresponding to each voltage component in the table below

 \setlength{\extrarowheight}{3mm}
 \begin{table}[h]
   \caption{In               the                last               step
     $     \mathbf{I_0}=V_0\frac{k}{\omega     l}=V_0\frac{1}{v     l}     =
     V_0\frac{\sqrt{lc}}{l} = V_0\sqrt{\frac{c}{l}}=V_0/Z_0 $.}
   \hspace*{-2.5cm}
   \begin{tabular}{|c|c|c|c|c|c|c|c|}
     \hline
     \textbf{Component} & {Voltage}, $ V $ & \multirow{4}{1.5ex}{$ \Rightarrow $}& $ \frac{dV}{dx} \equiv -l\frac{dI}{dt}$ &\multirow{4}{1.5ex}{$ \Rightarrow $}&  $ \frac{dI}{dt} $ &\multirow{4}{1.5ex}{$ \Rightarrow $}&  Current $ I $ \\\cline{1-2}\cline{4-4}\cline{6-6}\cline{8-8}
     $ \text{Left}\ + $ & $ \mathbf{V_0e^{ikx-i\omega t}} $ & & $ ikV_0e^{ikx-i\omega t} $ && $ -\frac{ik}{l}V_0e^{ikx-i\omega t} $ && $ \frac{k}{\omega l}V_0e^{ikx-i\omega t}  = \mathbf{I_0e^{ikx-i\omega t}}$\\\cline{1-2}\cline{4-4}\cline{6-6}\cline{8-8}
     $ \text{Left}\ - $ & $ \mathbf{rV_0e^{\red{-}ikx-i\omega t}} $ & & $ -ikrV_0e^{\red{-}ikx-i\omega t} $ && $ \frac{ik}{l}rV_0e^{\red{-}ikx-i\omega t} $ && $ -\frac{k}{\omega l}rV_0e^{\red{-}ikx-i\omega t}  = \mathbf{-rI_0e^{\red{-}ikx-i\omega t}}$\\\cline{1-2}\cline{4-4}\cline{6-6}\cline{8-8}
     $ \text{Right}\ + $ & $\mathbf{ tV_0e^{ikx-i\omega t}} $ & & $ iktV_0e^{ikx-i\omega t} $ && $ \frac{ik}{l}tV_0e^{ikx-i\omega t} $ && $ \frac{k}{\omega l}tV_0e^{ikx-i\omega t}  = \mathbf{tI_0e^{ikx-i\omega t}}$\\\hline
   \end{tabular}
 \end{table}

 \newpage
 Now, the equality of the currents and voltages on the two sides of the
 gap at  $ x=0  $ \red{\textbf{and  including the  potential difference
     drop                across                 the                gap,
     $      V_{\text{drop}}       =      I_{R}^{+}Z_{\text{gap}}      =
     \frac{tI_0e^{-i\omega t}}{i\omega  C_{\text{gap}}} $,  that causes
     the current on the other side of the gap}}

 \begin{equation}
   \left\lbrace\begin{aligned}
       I_0 e^{-i\omega t}-rI_0e^{-i\omega t} & = tI_0e^{-i\omega t}\\
       V_0 e^{-i\omega t}+rV_0e^{-i\omega t} & = tV_0e^{-i\omega t}+\frac{tI_0}{i\omega C_\text{gap}}\\
     \end{aligned}\right.\Rightarrow
   \left\lbrace\begin{aligned}
       1-r & =t\\
       1+r & = \bigg(1+\frac{1}{i\omega C_{\text{gap}}Z}\bigg)t
     \end{aligned}\right.
 \end{equation}

 \noindent and one can simply solve for $ r $ and $ t $ coefficients

 \begin{equation}\label{tLinert}
   \mathbf{\red{t= \frac{1}{1+\frac{1}{i2\omega C_\text{gap}Z}} = \frac{i\alpha}{1+i\alpha};\quad	 r = \frac{1}{1+i\alpha};\quad \alpha = 2\omega C_\text{gap}Z.}}
 \end{equation}

 \begin{figure}
   \centering%
   \includegraphics[height=3cm]{gap}
 \end{figure}

 Now suppose that we defined another  gap further down the line. Let us
 see what the resulting  voltage at $ x=L $ would  be. The voltage that
 is transmitted across the gap initially is $ tV_0 $

 \begin{multline}\label{tlineMUltiple}
   tV_0 \rightarrow \left\lbrace \text{travels $ L $ to
       $    x=L    $}\right\rbrace    \rightarrow   tV_0e^{ikL-i\omega    t}    \\
   \rightarrow\left\lbrace \text{reflects,  travels $ L  $ to $  x=0 $,
       reflects,  travels  L  to   $  x=L  $  }\right\rbrace\rightarrow
   r^2tV_0e^{ik3L-i\omega t}\\  \rightarrow\left\lbrace \text{reflects,
       travels $ L $ to $ x=0 $, reflects, travels L to $ x=L $
     }\right\rbrace\rightarrow     r^4tV_0e^{ik5L-i\omega      t}     \\
   \rightarrow\left\lbrace \text{reflects,  travels $ L  $ to $  x=0 $,
       reflects,  travels  L  to   $  x=L  $  }\right\rbrace\rightarrow
   r^6tV_0e^{ik7L-i\omega t} \\ \rightarrow\cdots
 \end{multline}

 \noindent so that the total voltage

 \begin{equation}\label{tlineTotalVoltage}
   \begin{aligned}
     V(x=L) & = tV_0e^{ikL-i\omega t}\bigg(1+r^2e^{i2kL}+r^4e^{i4kL}+r^6e^{i6kL}+\cdots\bigg)\\
     & = tV_0e^{ikL-i\omega t}\sum_{n=0}^{\infty}\bigg(r^2e^{2ikL}\bigg)^n, \quad\text{and since $ r<1 $ this is a convergent power series}\\
     & = \mathbf{\frac{tV_0e^{ikL-i\omega t}}{1-r^2e^{2ikL}}.}
   \end{aligned}
 \end{equation}

 \noindent To make good use of this, we need to use

 \begin{equation}\label{tlineApprox}
   \left\lbrace
     \begin{aligned}
       e^{i\alpha+i\alpha^2/2} & = 1+i\alpha +O(\alpha^3) \text{ (proof by simple expansion)}\\
       r & = (1+i\alpha)^{-1} \text{ (from before)}
     \end{aligned}\right.\Rightarrow r^2 \approx e^{-i2\alpha +\alpha^2}
 \end{equation}

 \noindent \red{This  and further mathematical  stuff will lead  to the
   voltage inside the resonator to be}

 \begin{equation}\label{tlineVoltage}
   V_r = \frac{V_0}{\alpha}\frac{i(-1)^{n}e^{-i\omega t}}{1+i\frac{2\delta\omega}{\Delta\omega}};\quad \Delta\omega = 2\alpha^2f_0;\quad \delta\omega = \text{ offset from $ n^{th} $ resonance}.
 \end{equation}

 \noindent  \red{As  can  be  seen,  the  maximum  voltage  inside  the
   resonator is $ 1/\alpha $ times  larger than the external field - we
   have boosted the  total field from the  combination of reflections.}
 In a similar way the voltage/power leaving the resonator are

 \begin{equation}\label{tlineLeaving}
   V_{out} = tV_r = \frac{V_0}{\alpha}\frac{i(-1)^{n+1}e^{-i\omega t}}{1+i\frac{2\delta\omega}{\Delta\omega}}; \quad P_{out} = \frac{P_0}{1+\left(\frac{2\delta\omega}{\Delta\omega}\right)^2}.
 \end{equation}

  \begin{figure}[h]
    \centering%
    \includegraphics[height=3cm]{gap1}
  \end{figure}


  \red{Important is  the quality factor  of the resonator. This  is the
    ratio  of the  resonance frequency  to the  width of  the resonance
    peak}

  \red{\begin{equation}\label{key}                  Q                 =
      \frac{\omega_{\text{resonance}}}{\Delta\omega}=\frac{\pi}{\left(2\omega
          ZC_{gap}\right)^2}.
    \end{equation}}

   \begin{figure}[h]
     \centering%
     \includegraphics[height=3cm]{res}
   \end{figure}

   Using      results     of      Table.\ref{tab:conversion2},     with
   $      V      =       V_0\bigg(a+a^\dagger\bigg);\quad      I      =
   iI_0\bigg(a-a^\dagger\bigg) $,  and the  results from  the classical
   resonator
   $ V=V_0\cos(\frac{\pi  n}{L}x);\quad I=I_0\sin(\frac{\pi n}{L}x)  $, the
   quantum field is

   \begin{align}
     \hat{V} & = \sqrt{\frac{\hbar\omega}{2c}}\bigg(a+a^\dagger\bigg)\cos(\frac{\pi n}{L}x)\\
     \hat{I} & = i\sqrt{\frac{\hbar\omega}{2l}}\bigg(a-a^\dagger\bigg)\sin(\frac{\pi n}{L}x)\\
   \end{align}

   \noindent and the total energy, given by the Hamiltonian is

   \begin{equation}\label{tlineTOtalGamil}
     \begin{aligned}
       \mathcal{H} & = \frac{1}{L}\int_{0}^{L}\bigg(\frac{l\hat{I}^2}{2}+\frac{c\hat{V}^2}{2}\bigg)dx \\
       & = \frac{l}{2}\frac{-\hbar\omega}{2l}\bigg(a-a^{\dagger}\bigg)^2\frac{1}{L}\int_{0}^{L}\cos^2(\frac{\pi n}{L}x)dx + \frac{c}{2}\frac{\hbar\omega}{2c}\bigg(a+a^{\dagger}\bigg)^2\frac{1}{L}\int_{0}^{L}\sin^2(\frac{\pi n}{L}x)dx\\
       & = -\frac{\hbar\omega}{4}\frac{1}{2}\bigg(aa-aa^{\dagger}-a^{\dagger}a+a^{\dagger}a^{\dagger}\bigg)+\frac{\hbar\omega}{4}\frac{1}{2}\bigg(aa+aa^{\dagger}+a^{\dagger}a+a^{\dagger}a^{\dagger}\bigg)\\
       &        =       \frac{\hbar\omega}{8}\bigg(aa^{\dagger}+a^{\dagger}a\bigg)=
       \frac{\hbar\omega}{8}\bigg((a^{\dagger}a+1)+a^{\dagger}a\bigg)=\mathbf{\hbar\omega\bigg(\hat{N}+\frac{1}{2}\bigg)},
     \end{aligned}
   \end{equation}

   \noindent so the resonator is a quantum harmonic oscillator.

   \newpage
